\documentclass[12pt]{article}
\usepackage[margin=1in]{geometry} 
\usepackage{amsmath,amsthm,amssymb,amsfonts,mathtools}

\newenvironment{problem}[2][]{
    \begin{trivlist}
        \item[
            {\bfseries #1}
            {\bfseries #2.}
        ]
}{\end{trivlist}}

\pagenumbering{gobble}

% --------------------------------------------------
% CUSTOM COMMANDS
% -------------------------------------------------- 

\newcommand{\assignment}{Pg. 456 \#15-29 odd, 32, 33-37 odd}
\newcommand{\name}{Eric Nguyen}
\newcommand{\duedate}{2019-03-19}
\newcommand{\details}{\temtbf{\\\name \\\duedate \\\assignment}}

\newcommand{\plugin}[2]{\left(\left({#1}\right) - \left({#2}\right)\right)}
\newcommand{\setuv}[4]{
\left[
\begin{alignedat}{2}
u &= #1 &\quad v &= #2 \\
du &= #3 &\quad dv &= #4 \\
\end{alignedat}
\right]  = uv - \int v ~ du \\
&= \intbp{#1}{#2}{#3}
}
\newcommand{\subu}[2]{
\left[
\begin{alignedat}{1}
u &= #1 \\
du &= #2 \\
\end{alignedat}
\right] 
}
\newcommand{\intbp}[3]{\left(#1\right) \left(#2\right) - \int \left(#2\right) \left(#3\right)}

% --------------------------------------------------  
% TABULAR INTEGRATION
% -------------------------------------------------- 

\usepackage{booktabs}
\usepackage{xparse}
\usepackage{tikz}
\usetikzlibrary{calc}

\tikzset{Arrow Style/.style={text=black, font=\boldmath}}

\newcommand{\tikzmark}[1]{%
    \tikz[overlay, remember picture, baseline] \node (#1) {};%
}

\newcommand*{\XShift}{0.5em}
\newcommand*{\YShift}{0.5ex}

\NewDocumentCommand{\DrawArrow}{s O{} m m m}{%
    \begin{tikzpicture}[overlay,remember picture]
        \draw[->, thick, Arrow Style, #2] 
                ($(#3.west)+(\XShift,\YShift)$) -- 
                ($(#4.east)+(-\XShift,\YShift)$)
        node [midway,above] {#5};
    \end{tikzpicture}%
}

\begin{document}

\details

\begin{problem}{15}
$\displaystyle\int m^3 \ln m ~ dm$
\begin{align}
&= m^{3 + 1} \left[\frac{\ln m}{3 + 1} - \frac{1}{\left(3 + 1\right)^2}\right] + C \\
&= m^4 \left[\frac{\ln m}{4} - \frac{1}{16}\right] + C \\
&= \frac{m^4}{4} \left(\ln m\right) - \frac{m^4}{16} + C
\end{align}
\end{problem}

\begin{problem}{17}
$\displaystyle\int \frac{dm}{\sqrt{m^2 + 7}}$
\begin{align}
&= \ln \left|m + \sqrt{m^2 + \sqrt{7}^2}\right| + C \\
&= \ln \left|m + \sqrt{m^2 + 7}\right| + C \\
\end{align}
\end{problem}

\begin{problem}{19}
$\displaystyle\int \frac{10 ~ dm}{m\left(5 - 7m\right)^2}$
\begin{align}
&= 10 \left(\frac{1}{5 \left(5 - 7m\right)} + \frac{1}{5^2} \ln \left|\frac{m}{5 - 7m}\right| + C\right) \\
&= \frac{2}{5 - 7m} + \frac{2}{5} \ln \left|\frac{m}{5 - 7m}\right| + C
\end{align}
\end{problem}

\begin{problem}{21}
$\displaystyle\int \frac{-5}{4m^2 - 1} ~ dm$
\begin{align}
&= -\frac{5}{4} \int \frac{1}{m^2 - \frac{1}{4}} ~ dm \\
&= -\frac{5}{4}\left(\frac{1}{2\left(\frac{1}{2}\right)} \ln\left|\frac{m - \frac{1}{2}}{m + \frac{1}{2}}\right| + C\right) \\
&= -\frac{5}{4} \ln\left|\frac{m - \frac{1}{2}}{m + \frac{1}{2}}\right| + C \\
\end{align}
\end{problem}

\begin{problem}{23}
$\displaystyle\int \sqrt{4m^2 + 16} ~ dm$
\begin{align}
&= 2 \int \sqrt{m^2 + 4} ~ dm \\
&= 2 \left(\frac{1}{2}\left[m\sqrt{m^2 + 4} + 4 \ln \left|m + \sqrt{m^2 + 4}\right|\right] + C\right) \\
&= m\sqrt{m^2 + 4} + 4 \ln \left|m + \sqrt{m^2 + 4}\right| + C
\end{align}
\end{problem}

\begin{problem}{25}
$\displaystyle\int \frac{-5 \ln x}{x^3} ~ dx$
\begin{align}
&= -5 \int x^{-3} \ln x ~ dx \\
&= -5 \left(x^{-3 + 1} \left[\frac{\ln x}{-3 + 1} - \frac{1}{\left(-3 + 1\right)^2}\right] + C\right) \\
&= -5x^{-2} \left[\frac{\ln x}{-2} - \frac{1}{4}\right] + C \\
&= \frac{5}{2x^2} \left(\ln x\right) + \frac{5}{4x^2} + C
\end{align}
\end{problem}

\begin{problem}{27}
$\displaystyle\int \frac{e^x}{x^{-3}} ~ dx$
\begin{align}
&= \int x^3 e^x ~ dx \\
&= \frac{x^3 e^x}{1} - \frac{3}{1} \int x^{3-1} e^x ~ dx + C \\
&= x^3 e^x - 3 \int x^2 e^x ~ dx + C \\
\int x^{2} e^x ~ dx &=
\renewcommand{\arraystretch}{1.5}
\begin{array}{c @{\hspace*{1.0cm}} c}
D & I \\
\cmidrule{1-2}
x^2\tikzmark{D1} & \tikzmark{I1}e^x \\
2x \tikzmark{D2} & \tikzmark{I2}e^{x} \\      
2 \tikzmark{D3} & \tikzmark{I3}e^{x} \\      
0 \tikzmark{D4} & \tikzmark{I4}e^{x}
\end{array} = x^2 e^x - 2x e^x + 2e^x + C \\
\int \frac{e^x}{x^{-3}} ~ dx &= x^3 e^x - 3 \left(x^2 e^x - 2xe^x + 2e^x\right) + C \\
&= x^3 e^x - 3x^2 e^x + 6x e^x - 6e^x + C
\end{align}
\DrawArrow{D1}{I2}{$+$}
\DrawArrow{D2}{I3}{$-$}
\DrawArrow{D3}{I4}{$+$}
\end{problem}

\begin{problem}{29}
$\displaystyle\int x \sqrt{1 + 2x} ~ dx$
\begin{align}
&= \frac{2}{15\left(2\right)^2} \left(3\left(2\right)x - 2\left(1\right)\right)\left(1 + 2x\right)^{3/2} + C \\
&= \frac{2}{60} \cdot 2 \left(3x - 1\right)\left(1 + 2x\right)^{3/2} + C \\
&= \frac{1}{15} \left(3x - 1\right)\left(1 + 2x\right)^{3/2} + C
\end{align}
\end{problem}

\begin{problem}{32}
$p'(t) = \frac{1}{t(2 + t)^2}, \quad p(2) = 0.8267$
\begin{align}
p(t) &= \frac{1}{2(2 + t)} + \frac{1}{4} \ln\left|\frac{t}{2 + t}\right| + C \\
0.8267 &= \frac{1}{2(2 + (2))} + \frac{1}{4} \ln\left|\frac{(2)}{2 + (2)}\right| + C \\
C &= \frac{1}{8} + \frac{1}{4} \ln\left|\frac{1}{2}\right| - 0.8267 \\
&\approx -0.875 \\
p(t) &= \frac{1}{2(2 + t)} + \frac{1}{4} \ln\left|\frac{t}{2 + t}\right| - 0.875
\end{align}
\end{problem}

\begin{problem}{33}
$\displaystyle\int \frac{8}{3x^2 - 2x} ~ dx$
\begin{align}
&= -8 \int \frac{1}{x(2 - 3x)} ~ dx \\
&= -8 \left(\frac{1}{2} \ln\left|\frac{x}{2 - 3x}\right| + C\right) \\
&= -4 \ln\left|\frac{x}{2 - 3x}\right| + C
\end{align}
\end{problem}

\begin{problem}{35}
$\displaystyle\int \frac{dx}{x^3 - 4x^2 + 4x}$
\begin{align}
&= \int \frac{1}{x(x - 2)^2} ~ dx \\
&= \frac{-1}{2(x - 2)} + \frac{1}{4} \ln\left|\frac{x}{x - 2}\right| + C
\end{align}
\end{problem}

\begin{problem}{37}
$\displaystyle\int \frac{-e^{-2x} ~ dx}{9 - 6e^{-x} + e^{-2x}}$
\begin{align}
&= - \int \frac{e^{-2x} ~ dx}{9 - 6e^{-x} + e^{-2x}} \\
&= \subu{e^{-x}}{-e^{-x} ~ dx} = \int \frac{u ~ du}{9 - 6u + u^2} \\
&= \int \frac{u ~ du}{(u - 3)^2} \\
&= \frac{-3}{1(u - 3)} + \frac{1}{1} \ln\left|u - 3\right| + C \\
&= \frac{-3}{(e^{-x} - 3)} + \ln\left|e^{-x} - 3\right| + C
\end{align}
\end{problem}

\end{document}
