\documentclass[12pt]{article}
\usepackage[margin=1in]{geometry} 
\usepackage{amsmath,amsthm,amssymb,amsfonts,mathtools}

\newenvironment{problem}[2][]{
    \begin{trivlist}
        \item[
            {\bfseries #1}
            {\bfseries #2.}
        ]
}{\end{trivlist}}

\pagenumbering{gobble}

\newcommand{\assignment}{Pg. 451 \#1-35 eoo, 39, 41, 49}
\newcommand{\name}{Eric Nguyen}
\newcommand{\duedate}{2019-03-19}
\newcommand{\details}{\textbf{\\\name \\\duedate \\\assignment}}

\newcommand{\plugin}[2]{\left(\left({#1}\right) - \left({#2}\right)\right)}
\newcommand{\setuv}[4]{
\left[
\begin{alignedat}{2}
u &= #1 &\quad v &= #2 \\
du &= #3 &\quad dv &= #4 \\
\end{alignedat}
\right]  = uv - \int v ~ du \\
&= \intbp{#1}{#2}{#3}
}
\newcommand{\subu}[2]{
\left[
\begin{alignedat}{1}
u &= #1 \\
du &= #2 \\
\end{alignedat}
\right] 
}
\newcommand{\intbp}[3]{\left(#1\right) \left(#2\right) - \int \left(#2\right) \left(#3\right)}

\begin{document}

\details

\begin{problem}{1}
$\displaystyle\int 4xe^{4x} ~ dx$
\begin{align}
&= \setuv{4x}{\frac{e^{4x}}{4}}{4 ~ dx}{e^{4x} ~ dx} \\
&= xe^{4x} - \frac{1}{4}e^{4x} + C
\end{align}
\end{problem}

\begin{problem}{5}
$\displaystyle\int xe^{5x} ~ dx$
\begin{align}
&= \setuv{x}{\frac{1}{5} e^{5x}}{dx}{e^{5x} ~ dx} \\
&= \frac{1}{5} xe^{5x} - \frac{1}{25} e^{5x} + C \\
\end{align}
\end{problem}

\begin{problem}{9}
$\displaystyle\int x^2 \ln \left(x + 5\right) dx$
\begin{align}
&= \setuv{\ln \left(x + 5\right)}{\frac{x^3}{3}}{\frac{1}{x} ~ dx}{x^2 ~ dx} \\
&= \frac{x^3 \ln \left(x + 5\right)}{3} - \frac{1}{3} \int x^2 ~ dx \\
&= \frac{x^3 \ln \left(x + 5\right)}{3} - \frac{x^3}{9} + C
\end{align}
\end{problem}

\begin{problem}{13}
$\displaystyle\int \ln\left(x + 5\right) dx$
\begin{align}
&= \subu{x + 5}{dx} = \int \ln \left(u\right) du \\
&= u \ln \left(u\right) - u + C \\
&= \left(x + 5\right) \ln \left(x + 5\right) - \left(x + 5\right) + C \\
&= \left(x + 5\right) \ln \left(x + 5\right) - x + C
\end{align}
\end{problem}

\begin{problem}{17}
$\displaystyle\int \left(x - 1\right) \ln x ~ dx$
\begin{align}
&= \setuv{\ln x}{\frac{x^2}{2} - x}{\frac{1}{x} ~ dx}{\left(x - 1\right) dx} \\
&= \frac{x^2 \ln x}{2} - x \ln x - \int \frac{x}{2} - 1 ~ dx \\
&= \frac{x^2 \ln x}{2} - x \ln x - \left(\frac{1}{2} \int x ~ dx - \int 1 ~ dx\right) \\
&= \left(\frac{x^2}{2} - x\right) \ln x - \frac{x^2}{4} + x + C \\
\end{align}
\end{problem}

\begin{problem}{21}
$\displaystyle\int x^3 \ln \left(2x\right) dx$
\begin{align}
&= \setuv{\ln \left(2x\right)}{\frac{x^4}{4}}{\frac{1}{x} ~ dx}{x^3 ~ dx} \\
&= \frac{x^4 \ln \left(2x\right)}{4} - \frac{1}{4} \int x^3 ~ dx \\
&= \frac{x^4}{4} \ln \left(2x\right) - \frac{x^4}{16} + C
\end{align}
\end{problem}

\begin{problem}{25}
$\displaystyle\int x^2e^{2x} ~ dx$
\begin{align}
&= \setuv{x^2}{\frac{e^{2x}}{2}}{2x ~ dx}{e^{2x} ~ dx} \\
&= \frac{1}{2} x^2e^{2x} - \int xe^{2x} ~ dx \\
\int xe^{2x} ~ dx &= \setuv{x}{\frac{e^{2x}}{2}}{dx}{e^2x ~ dx} \\
&= \frac{1}{2} xe^{2x} - \frac{1}{2} \int e^{2x} ~ dx \\
&= \frac{1}{2} xe^{2x} - \frac{1}{4}e^2x + C \\
&= \frac{1}{2} x^2e^{2x} - \left(\frac{1}{2} xe^{2x} - \frac{1}{4} e^2x\right) + C \\
&= \frac{1}{2} x^2e^{2x} - \frac{1}{2} xe^{2x} + \frac{1}{4} e^2x + C
\end{align}
\end{problem}

\begin{problem}{29}
$\displaystyle\int \left(x^4 + 4\right) e^{3x} ~ dx$
\begin{align}
&= \setuv{x^4 + 4}{\frac{e^3x}{3}}{4x^3 ~ dx}{e^{3x} ~ dx} \\
&= \frac{1}{3} x^4e^3x + \frac{4}{3} xe^3 - \frac{4}{3} \int x^4e^3 ~ dx \\
\int x^4e^3 ~ dx &= \setuv{x^4}{\frac{e^3}{3}}{4x^3 ~ dx}{e^3 ~ dx} \\
&= \frac{1}{3} x^4e^3 - \frac{4}{3} \int x^3 e^3 ~ dx \\
\int x^3e^3 ~ dx &= \setuv{x^3}{\frac{e^3}{3}}{3x^2 ~ dx}{e^3 ~ dx} \\
&= \frac{1}{3} x^3e^3 - \int x^2e^3 ~ dx \\
\int x^2e^3 ~ dx &= \setuv{x^2}{2x}{\frac{e^3}{3}}{e^3 ~ dx} \\
&= 2x^3 - \frac{2}{3} \int xe^3 ~ dx \\
\int xe^3 ~ dx &= \setuv{x}{\frac{e^3}{3}}{dx}{e^3 ~ dx} \\
&= \frac{1}{3} - \frac{e^3}{9} + C \\
\int \left(x^4 + 4\right) e^{3x} ~ dx &= \frac{1}{3} x^4e^3x + \frac{4}{3} xe^3 - \frac{4}{3} \left(\frac{1}{3} x^4e^3 - \frac{4}{3}\left(\frac{1}{3} x^3e^3 - \left(2x^3 - \frac{2}{3} \left(\frac{1}{3} - \frac{e^3}{9}\right)\right)\right)\right) + C
\end{align}
\end{problem}

\begin{problem}{33}
$\displaystyle\int_2^6 \ln \left(x + 8\right) dx$
\begin{align}
&= \setuv{\ln \left(x + 8\right)}{x}{\frac{1}{x + 8} ~ dx}{dx} \\
&= x \ln \left(x + 8\right) - \int \frac{x}{x + 8} ~ dx \\
\int \frac{x}{x+8} ~ dx &= \setuv{\frac{1}{x + 8}}{\frac{x^2}{2}}{-\frac{1}{x^2} ~ dx}{x ~ dx} \\
&= \frac{x^2}{2 \left(x + 8\right)} + \frac{1}{2} \int 1 dx \\
&= \frac{x^2}{2 \left(x + 8\right)} + \frac{x}{2} \\
\int_2^6 \ln \left(x + 8\right) dx &= x \ln \left(x + 8\right) - \left(\frac{x^2}{2 \left(x + 8\right)} + \frac{x}{2}\right) \bigg|_2^6
\end{align}
\end{problem}

\begin{problem}{39}
$K(t) = 10te^{-t}$
\begin{align}
\shortintertext{a)}
\int_0^T K(t) &= \setuv{10t}{-e^{-t}}{10 ~ dt}{e^{-t} ~ dt} \\
&= -10te^{-t} - 10e^{-t} ~ \bigg|_0^{T} \\
&= -10(T)e^{-(T)} - 10e^{-(T)} - \left(-10(0)e^{-(0)} - 10e^{-(0)}\right) \\
&= -10Te^{-T} - 10e^{-T} + 10 \\
\shortintertext{b)}
-10(4)e^{-(4)} - 10e^{-(4)} + 10 &\approx 9.084 ~ \text{kW-h}
\end{align}
\end{problem}

\begin{problem}{41}
$\displaystyle\int \sqrt{x} \ln x ~ dx$
\begin{align}
&= \setuv{\ln x}{\frac{2}{3} x^{3/2}}{\frac{1}{x} ~ dx}{\sqrt{x} ~ dx} \\
&= \frac{2}{3} x^{3/2} \ln x - \frac{2}{3} \int \sqrt{x} ~ dx \\
&= \frac{2}{3} x^{3/2} \ln x - \frac{4}{9} x^{3/2} + C
\end{align}
\end{problem}

\begin{problem}{49}
Verify that for any positive integer n, $\displaystyle\int x^ne^x ~ dx = x^ne^x - n \displaystyle\int x^{n - 1}e^x ~ dx$
\begin{align}
\int x^ne^x ~ dx &= \setuv{x^n}{e^x}{nx^{n - 1}}{e^x ~ dx} \\
&= x^ne^x - n \int x^{n - 1}e^x ~ dx
\end{align}
\end{problem}

\end{document}
