\documentclass[12pt]{article}
\usepackage[margin=1in]{geometry} 
\usepackage{amsmath,amsthm,amssymb,amsfonts,mathtools}

\newenvironment{problem}[2][]{
    \begin{trivlist}
        \item[
            {\bfseries #1}
            {\bfseries #2.}
        ]
}{\end{trivlist}}

\pagenumbering{gobble}

\newcommand{\assignment}{Pg. 442 \#15, 31, 43-51 eoo, 63, 67, 69, 82, 87}
\newcommand{\name}{Eric Nguyen}
\newcommand{\duedate}{2019-03-15}
\newcommand{\details}{\textbf{\\\name \\\duedate \\\assignment}}

\newcommand{\plugin}[2]{\left(\left({#1}\right) - \left({#2}\right)\right)}

\begin{document}

\details

\begin{problem}{15}
$\displaystyle\int x^4 e^{x^5} ~ dx$
\begin{align}
u &= x^5 \\
\frac{du}{dx} &= 5x^4 \\
du &= 5x^4 ~ dx \\
\frac{1}{5} ~ du &= x^4 ~ dx \\
\int x^4 e^{x^5} &= \int e^u \cdot \frac{1}{5} ~ du \\
&= \frac{1}{5} e^u + C \\
&= \frac{1}{5} e^{x^5} + C
\end{align}
\end{problem}

\begin{problem}{31}
$\displaystyle\int \frac{(\ln x)^2}{x} ~ dx$
\begin{align}
u &= \ln x \\
\frac{du}{dx} &= \frac{1}{x} \\
du &= \frac{1}{x} ~ dx \\
\int \frac{(\ln x)^2}{x} ~ dx &= \int u^2 ~ du \\
&= \frac{u^3}{3} + C \\
&= \frac{(\ln x)^3}{3} + C
\end{align}
\end{problem}

\begin{problem}{43}
$\displaystyle\int_0^1 2xe^{x^2} ~ dx$
\begin{align}
u &= x^2 \\
\frac{du}{dx} &= 2x \\
du &= 2x ~ dx \\
\int_0^1 2xe^{x^2} ~ dx &= \int_0^1 e^u ~ du \\
&= e^u ~ \bigg|_0^1 \\
&= e^{x^2} ~ \bigg|_0^1 \\
&= \plugin{e^{(1)^2}}{e^{(0)^2}} \\
&= e - 1
\end{align}
\end{problem}

\begin{problem}{47}
$\displaystyle\int_0^4 \frac{dt}{1 + t}$
\begin{align}
u &= 1 + t \\
\frac{du}{dt} &= 1 \\
du &= dt \\
\int_0^4 \frac{dt}{1 + t} &= \int_0^4 \frac{du}{u} \\
&= \ln u ~ \bigg|_0^4 \\
&= \ln{\left(1 + t\right)} ~ \bigg|_0^4 \\
&= \plugin{\ln{\left(1 + (4)\right)}}{\ln{\left(1 + (0)\right)}} \\
&= \ln 5
\end{align}
\end{problem}

\begin{problem}{51}
$\displaystyle\int_0^b e^{-x} ~ dx$
\begin{align}
&= -e^{-x} ~ \bigg|_0^b \\
&= \plugin{-e^{-(b)}}{-e^{-(0)}} \\
&= -e^{-b} + 1 \\
&= 1 - e^{-b}
\end{align}
\end{problem}

\begin{problem}{63}
$R'(t) = 4000t, \quad V(t) = 200,000 - 25,000e^{0.1t}, \quad R(0) = 0$
\begin{align}
\shortintertext{a) Find P(t)}
P(t) &= R(t) + V(t) - 250,000 \\
&= 2000t^2 + 200,000 - 25,000e^{0.1t} - 250,000 \\
&= 2000t^2 - 50,000 - 25,000e^{0.1t}
\shortintertext{b) Find P(10)}
P(10) &= 2000(10)^2 - 50,000 - 25,000e^{0.1(10)} \\
&= \$82,042.95
\end{align}
\end{problem}

\begin{problem}{69}
$\displaystyle\int 5x \sqrt{1 - 4x^x} ~ dx$
\begin{align}
u &= 1 - 4x^2 \\
\frac{du}{dx} &= -8x \\
-\frac{5}{8} ~ du &= 5x ~ dx \\
\int 5x \sqrt{1 - 4x^2} ~ dx &= \int -\frac{5}{8} \sqrt{u} ~ du \\
&= -\frac{5}{8} \int \sqrt{u} ~ du \\
&= -\frac{5}{8} \cdot \frac{2}{3} u^{3/2} + C \\
&= -\frac{5}{12} (1 - 4x^2)^{3/2} + C
\end{align}
\end{problem}

\begin{problem}{82}
$\displaystyle\int \frac{x^2 + 6x}{(x + 3)^2} ~ dx$
\begin{align}
&= \int \frac{x^2 + 6x + 9 - 9}{x^2 + 6x + 9} ~ dx \\
&= \int \frac{x^2 + 6x + 9}{x^2 + 6x + 9} - \frac{9}{x^2 + 6x + 9} ~ dx \\
&= \int 1 ~ dx - 9 \int \frac{1}{(x + 3^2)} ~ dx \\
u &= x + 3 \\
du &= dx \\
\int \frac{x^2 + 6x}{(x + 3)^2} ~ dx &= x - 9 \int \frac{1}{u^2} ~ du \\
&= x + 9 \frac{1}{u} + C \\
&= x + \frac{9}{x + 3} + C
\end{align}
\end{problem}

\begin{problem}{87}
$\displaystyle\int \frac{e^x - e^{-x}}{e^x + e^{-x}} ~ dx$
\begin{align}
u &= e^x + e^{-x} \\
\frac{du}{dx} &= e^x - e^{-x} \\
\int \frac{e^x - e^{-x}}{e^x + e^{-x}} ~ dx &= \int \frac{1}{u} ~ du \\
&= \ln{u} + C \\
&= \ln{e^x + e^{-x}} + C
\end{align}
\end{problem}

\end{document}