\documentclass[12pt]{article}
\usepackage[margin=1in]{geometry} 
\usepackage{amsmath,amsthm,amssymb,amsfonts}
 
\newenvironment{problem}[2][]{
    \begin{trivlist}
        \item[
            {\bfseries #1}
            {\bfseries #2.}
        ]
}{\end{trivlist}}

\pagenumbering{gobble}

\newcommand{\assignment}{Pg. 409 \#1-58 eoo, 67, 69, 73, 75, 79}
\newcommand{\name}{Eric Nguyen}
\newcommand{\duedate}{2019-02-11}
\newcommand{\details}{\textbf{\\\name \\\duedate \\\assignment}}
 
\begin{document}

\details

\begin{problem}{1}
$\displaystyle\int x^6 \, dx$
\begin{align}
&= \dfrac{x^7}{7} + C
\end{align}
\end{problem}

\begin{problem}{5}
$\displaystyle\int x^{1/4} \, dx$
\begin{align}
&= \dfrac{x^{5/4}}{5/4} + C \\
&= \dfrac{4}{5} x^{5/4} + C
\end{align}
\end{problem}

\begin{problem}{9}
$\displaystyle\int (2t^2 + 5t - 3) \, dt$
\begin{align}
&= \int 2t^2 \, dt + \int 5t \, dt - \int 3 \, dt \\ 
&= 2 \int t^2 \, dt + 5 \int t \, dt - 3t + C \\
&= 2 \cdot \dfrac{t^3}{3} + 5 \cdot \dfrac{t^2}{2} - 3t + C \\
&= \dfrac{2}{3}t^3 + \dfrac{5}{2}t^2 - 3t + C
\end{align}
\end{problem}

\begin{problem}{13}
$\displaystyle\int \sqrt[\scriptstyle 3]{x} \, dx$
\begin{align}
&= \int x^{1/3} \, dx \\
&= \dfrac{x^{4/3}}{4/3} + C \\
&= \dfrac{3}{4} x^{4/3} + C
\end{align}
\end{problem}

\begin{problem}{17}
$\displaystyle\int \dfrac{dx}{x^4}$
\begin{align}
&=  \int x^{-4} \, dx \\
&=  -\dfrac{1}{3} x^{-3} + C
\end{align}
\end{problem}

\begin{problem}{21}
$\displaystyle\int \left(\dfrac{3}{x} + \dfrac{5}{x^2}\right) \, dx$
\begin{align}
&= \int \dfrac{3}{x} \, dx + \int \dfrac{5}{x^2} \, dx \\
&= 3 \int \dfrac{1}{x} \, dx + 5 \int x^{-2} \, dx \\
&= 3 \ln{\left|x\right|} - 5x^{-1} + C
\end{align}
\end{problem}

\begin{problem}{25}
$\displaystyle\int 2e^{2x} \, dx$
\begin{align}
&= 2 \int e^{2x} \, dx \\
&= 2 \cdot \dfrac{1}{2} e^{2x} + C \\
&= e^{2x} + C
\end{align}
\end{problem}

\begin{problem}{29}
$\displaystyle\int e^{7x} \, dx$
\begin{align}
&= \dfrac{1}{7} e^{7x} + C
\end{align}
\end{problem}

\begin{problem}{33}
$\displaystyle\int 6e^{8x} \, dx$
\begin{align}
&= 6 \int e^{8x} \, dx \\
&= \dfrac{6}{8} e^{8x} + C \\
&= \dfrac{3}{4} e^{8x} + C
\end{align}
\end{problem}

\begin{problem}{37}
$\displaystyle\int (5x^2 - 2e^{7x}) \, dx$
\begin{align}
&= \int 5x^2 \, dx - \int 2e^{7x} \, dx \\
&= 5 \int x^2 \, d - 2 \int e^{7x} \, dx \\
&= 5 \cdot \dfrac{1}{3} x^3 - 2 \cdot \dfrac{1}{7} e^{7x} + C \\
&= \dfrac{5}{3} x^3 - \dfrac{2}{7} e^{7x} + C
\end{align}
\end{problem}

\begin{problem}{41}
$\displaystyle\int (3x + 2)^2 \, dx$
\begin{align}
&= \int (3x + 2)(3x + 2) \, dx \\
&= \int 9x^2 + 6x + 6x + 4 \, dx \\
&= \int 9x^2 \, dx + \int 12x \, dx + \int 4 \, dx \\
&= 9 \int x^2 \, dx + 12 \int x \, dx + 4x + C \\
&= 9 \cdot \dfrac{1}{3} x^3 + 12 \cdot \dfrac{1}{2} x^2 + 4x + C \\
&= 3x^3 + 6x^2 + 4x + C
\end{align}
\end{problem}

\begin{problem}{45}
$\displaystyle\int \left(\dfrac{7}{\sqrt{x}} - \dfrac{2}{3} e^{5x} - \dfrac{8}{x}\right)$
\begin{align}
&= \int \dfrac{7}{\sqrt{x}} \, dx - \int \dfrac{2}{3} e^{5x} \, dx - \int \dfrac{8}{x} \, dx \\
&= 7 \int x^{-1/2} \, dx - \dfrac{2}{3} \int e^{5x} \, dx - 8 \int \dfrac{1}{x} \, dx \\
&= 7 \cdot 2\sqrt{x} - \dfrac{2}{3} \cdot \dfrac{1}{5} e^{5x} - 8 \ln{|x|} + C \\
&= 14\sqrt{x} - \dfrac{2}{15} e^{5x} - 8 \ln{|x|} + C 
\end{align}
\end{problem}

\begin{problem}{49}
$f'(x) = x^2 - 4, \quad f(0) = 7$
\begin{align}
f(x) &= \int x^2 - 4 \, dx \\
&= \int x^2 \, dx - \int 4 \, dx \\
&= \dfrac{1}{3} x^3 - 4x + C \\
\dfrac{1}{3} (0)^3 + C &= 7 \\
C &= 7 \\
f(x) &= \dfrac{1}{3} x^3 - 4x + 7
\end{align}
\end{problem}

\begin{problem}{53}
$f'(x) = 3x^2 - 5x + 1, \quad f(1) = \dfrac{7}{2}$
\begin{align}
f(x) &= \int 3x^2 - 5x + 1 \, dx \\
&= \int 3x^2 \, dx - \int 5x \, dx + \int 1 \, dx \\
&= 3 \int x^2 \, dx - 5 \int x \, dx + x + C \\
&= 3 \cdot \dfrac{1}{3} x^3 - 5 \cdot \dfrac{1}{2} x^2 + x + C \\
&= x^3 - \dfrac{5}{2} x^2 + x + C \\
(1)^3 - \dfrac{5}{2} (1)^2 + (1) + C &= \dfrac{7}{2} \\
C &= \dfrac{7}{2} - 1 + \dfrac{5}{2} - 1 \\
C &= 4 \\
f(x) &= x^3 - \dfrac{5}{2} x^2 + x + 4
\end{align}
\end{problem}

\begin{problem}{57}
$f'(x) = \dfrac{4}{\sqrt{x}}, \quad f(1) = -5$
\begin{align}
f(x) &= \int \dfrac{4}{\sqrt{x}} \, dx \\
&= 4 \int x^{-1/2} \, dx \\
&= 4 \cdot 2 \sqrt{x} + C \\
&= 8 \sqrt{x} + C \\
8 \sqrt{(1)} + C &= -5 \\
C &= -5 - 8 \\
C &= -13 \\
f(x) &= 8 \sqrt{x} - 13
\end{align}
\end{problem}

\newpage

\begin{problem}{67}
$\dfrac{dE}{dt} = 30 - 10t$
\end{problem}

\begin{problem}{a)}
$E(2) = 72$
\begin{align}
E(t) &= \int 30 - 10t \, dt \\
&= \int 30 \, dt - \int 10t \, dt \\
&= 30t - 10 \int t \, dt + C \\
&= 30t - 10 \cdot \dfrac{1}{2} t^2 + C \\
&= 30t - 5t^2 + C \\
30(2) - 5(2)^2 + C &= 72 \\
60 - 20 + C &= 72 \\
C &= 72 - 40 \\
C &= 32 \\
E(t) &= 30t - 5t^2 + 32 
\end{align}
\end{problem}

\begin{problem}{b)}
Find $E(3)$ and $E(5)$, where $E$ is a percentage.
\begin{align}
E(3) &= 30(3) - 5(3)^2 + 32 \\
&= 77\% \\
E(5) &= 30(5) - 5(5)^2 + 32 \\
&= 57\%
\end{align}
\end{problem}

\begin{problem}{69}
$I'(t) = 3.389e^{0.1049t}$
\end{problem}

\begin{problem}{a)}
$I(0) = 0$
\begin{align}
I(t) &= \int 3.389e^{0.1049t} \, dt \\
&= 3.389 \int e^{0.1049t} \, dt \\
&= 3.389 \cdot \dfrac{1}{0.1049} e^{0.1049t} + C \\
&\approx 32.31e^{0.1049t} + C \\
32.31e^{0.1049(0)} + C &\approx 0 \\
C &\approx 32.31 \\
I(t) &\approx 32.31e^{0.1049t} - 32.31
\end{align}
\end{problem}

\begin{problem}{b)}
$I(27)$
\begin{align}
&= 32.31e^{0.1049(27)} - 32.31 \\
&\approx 516 \text{ people}
\end{align}
\end{problem}

\begin{problem}{c)}
$I(34)$
\begin{align}
&= 32.31e^{0.1049(34)} - 32.31 \\
&\approx 1111 \text{ people}
\end{align}
\end{problem}

\begin{problem}{d)}
$I(34) - I(34 - 7)$
\begin{align}
&\approx 1111 - 32.31e^{0.1049(34 - 7)} - 32.31 \\
&\approx 1111 - 516 \\
&\approx 595 \text{ people}
\end{align}
\end{problem}

\begin{problem}{73}
$\displaystyle\int (5t + 4)^2 t^4 \, dt$
\begin{align}
&= \int (5t + 4)(5t + 4)t^4 \, dt \\
&= \int (25t^2 + 20t + 20t + 16)t^4 \, dt \\
&= \int 25t^6 + 40t^5 + 16t^4 \, dt \\
&= \int 25t^6 \, dt + \int 40t^5 \, dt + \int 16t^4 \, dt \\
&= 25 \int t^6 \, dt + 40 \int t^5 \, dt + 16 \int t^4 \, dt \\
&= 25 \cdot \dfrac{1}{7} t^7 + 40 \cdot \dfrac{1}{6} t^6 + 16 \cdot \dfrac{1}{5} t^5 + C \\
&= \dfrac{25}{7} t^7 + \dfrac{20}{3} t^6 + \dfrac{16}{5} t^5 + C
\end{align}
\end{problem}

\begin{problem}{75}
$\displaystyle\int (1 - t) \sqrt{t} \, dt$
\begin{align}
&= \int \sqrt{t} - t \sqrt{t} \, dt \\
&= \int t^{1/2} \, dt - \int t^{3/2} \, dt \\
&= \dfrac{2}{3} t^{3/2} - \dfrac{2}{5} t^{5/2} + C
\end{align}
\end{problem}

\begin{problem}{79}
$\displaystyle\int \dfrac{1}{\ln{10}} \dfrac{dx}{x}$
\begin{align}
&= \dfrac{1}{\ln{10}} \int \dfrac{1}{x} \, dx \\
&= \dfrac{\ln{|x|}}{\ln{10}} + C, \text{ or } \log{x} + C
\end{align}
\end{problem}

\end{document}