\documentclass[12pt]{article}
\usepackage[margin=1in]{geometry} 
\usepackage{amsmath,amsthm,amssymb,amsfonts,mathtools}

\newenvironment{problem}[2][]{
    \begin{trivlist}
        \item[
            {\bfseries #1}
            {\bfseries #2.}
        ]
}{\end{trivlist}}

\pagenumbering{gobble}

\newcommand{\assignment}{Pg. 433 \#3, 5, 11, 15, 16, 17, 23, 29, 33, 35, 53, 60}
\newcommand{\name}{Eric Nguyen}
\newcommand{\duedate}{2019-02-27}
\newcommand{\details}{\textbf{\\\name \\\duedate \\\assignment}}

\newcommand{\plugin}[2]{\left(\left({#1}\right) - \left({#2}\right)\right)}
\newcommand{\defint}[3]{\int_{#1}^{#2} #3}
\newcommand{\inteval}[3]{\left.#3\right|_{#1}^{#2}}

\newcommand{\descmeet}{\shortintertext{Find where the graphs meet:}}
\newcommand{\deschigh}{\shortintertext{Find the graph that is higher between the interval:}}
\newcommand{\descarea}{\shortintertext{Find the area of the difference of the two graphs between the interval:}}

\begin{document}

\details

\begin{problem}{3}
$
g(x) = \begin{cases} 
x^2 + 4, &\quad \text{for} \quad x \leq 0, \\
4 - x, &\quad \text{for} \quad x > 0
\end{cases}
$
\begin{align}
\defint{-2}{3}{g(x)} &= \defint{-2}{0}{x^2 + 4} + \defint{0}{3}{4 - x} \\
&= \inteval{-2}{0}{\frac{x^3}{3} + 4x} + \inteval{0}{3}{4x - \frac{x^2}{2}} \\
&= \plugin{\frac{(0)^3}{3} + 4(0)}{\frac{(-2)^3}{3} + 4(-2)} \notag \\
&\quad + \plugin{4(3) - \frac{(3)^2}{2}}{4(0) - \frac{(0)^2}{2}} \\
&= 18 \frac{1}{6}
\end{align}
\end{problem}

\begin{problem}{5}
$
f(x) = \begin{cases}
-x^2 - 6x + 7, &\quad \text{for} \quad x < 1 \\
\frac{3}{2}x - 1, &\quad \text{for} \quad x \geq 1
\end{cases}
$
\begin{align}
\defint{-6}{4}{f(x)} &= \defint{-6}{1}{-x^3 - 6x + 7} + \defint{1}{4}{\frac{3}{2}x - 1} \\
&= \inteval{-6}{1}{-\frac{x^3}{3} - 3x^2 + 7x} + \inteval{1}{4}{\frac{3x^2}{4} - x} \\
&= \plugin{-\frac{(1)^3}{3} - 3(1)^2 + 7(1)}{-\frac{(-6)^3}{3} - 3(-6)^2 + 7(-6)} \notag \\
&\quad + \plugin{\frac{3(4)^2}{4} - (4)}{\frac{3(1)^2}{4} - (1)} \\
&= 89 \frac{11}{12}
\end{align}
\end{problem}

\begin{problem}{11}
$f(x) = x^2 - x - 5, \quad g(x) = x + 10$
\begin{align}
x^2 - x - 5 &= x + 10 \\
x^2 - 2x - 15 &= 0 \\
(x + 3)(x - 5) &= 0 \\
x &= -3, 5
\end{align}
\end{problem}

\begin{problem}{15}
$f(x) = x^4 - 8x^3 + 18x^2, \quad g(x) = x + 28$
\begin{align}
A &= \defint{-1}{4}{g(x)} - \defint{-1}{4}{f(x)} \\
&= \defint{-1}{4}{x + 28} - \defint{-1}{4}{x^4 - 8x^3 + 18x^2} \\
&= \inteval{-1}{4}{\frac{x^2}{2} + 28x} - \inteval{-1}{4}{\frac{x^5}{5} - 2x^4 + 6x^3} \\
&= \plugin{\frac{(4)^2}{2} + 28(4)}{\frac{(-1)^2}{2} + 28(-1)} \notag \\
&\quad - \plugin{\frac{(4)^5}{5} - 2(4)^4 + 6(4)^3}{\frac{(-1)^5}{5} - 2(-1)^4 + 6(-1)^3} \\
&= 62.5
\end{align}
\end{problem}

\begin{problem}{16}
$f(x) = 4x - x^2, \quad g(x) = x^2 - 6x + 8$
\begin{align}
A &= \defint{1}{4}{f(x)} - \defint{1}{4}{g(x)} \\
&= \defint{1}{4}{4x - x^2} - \defint{1}{4}{x^2 - 6x + 8} \\
&= \inteval{1}{4}{2x^2 - \frac{x^3}{3}} - \inteval{1}{4}{\frac{x^3}{3} - 3x^2 + 8x} \\
&= \plugin{2(4)^2 - \frac{(4)^3}{3}}{2(1)^2 - \frac{(1)^3}{3}} \notag \\
&\quad - \plugin{\frac{(4)^3}{3} - 3(4)^2 + 8(4)}{\frac{(1)^3}{3} - 3(1)^2 + 8(1)} \\
&= 9
\end{align}
\end{problem}

\begin{problem}{17}
$y = x, \quad y = x^3, \quad x = 0, \quad x = 1$
\begin{align}
A &= \defint{0}{1}{x} - \defint{0}{1}{x^3} \\
&= \inteval{0}{1}{\frac{x^2}{2}} - \inteval{0}{1}{\frac{x^4}{4}} \\
&= \plugin{\frac{(1)^2}{2}}{\frac{(0)^2}{2}} - \plugin{\frac{(1)^4}{4}}{\frac{(0)^4}{4}} \\
&= \frac{1}{4}
\end{align}
\end{problem}

\clearpage

\begin{problem}{23}
$y = 2x - x^2, \quad y = -x$
\begin{align}
\descmeet
2x - x^2 &= -x \\
3x - x^2 &= 0 \\
x(3 - x) &= 0 \\
x &= 0, 3 \\
\deschigh
2(1) - (1)^2 &= 1 \\
-(1) &= -1 \\
\descarea
A &= \defint{0}{3}{2x - x^2} - \defint{0}{3}{-x} \\
&= \inteval{0}{3}{x^2 - \frac{x^3}{3}} - \inteval{0}{3}{-\frac{x^2}{2}} \\
&= \plugin{(3)^2 - \frac{(3)^3}{3}}{(0)^2 - \frac{(0)^3}{3}} - \plugin{-\frac{(3)^2}{2}}{-\frac{(3)^2}{2}} \\
&= 4 \frac{1}{2}
\end{align}
\end{problem}

\begin{problem}{29}
$y = 4 - x^2, \quad y = 4 - 4x$
\begin{align}
\descmeet
4 - x^2 &= 4 - 4x \\
-x^2 + 4x &= 0 \\
-x(x - 4) &= 0 \\
x &= 0, 4
\deschigh
4 - (1)^2 &= 3 \\
4 - 4(1) &= 0 \\
\descarea
A &= \defint{0}{4}{4 - x^2} - \defint{0}{4}{4 - 4x} \\
&= \inteval{0}{4}{4x - \frac{x^3}{3}} - \inteval{0}{4}{4x - 2x^2} \\
&= \plugin{4(4) - \frac{(4)^3}{3}}{4(0) - \frac{(0)^3}{3}} - \plugin{4(4) - 2(4)^2}{4(0) - 2(0)^2} \\
&= 10 \frac{2}{3}
\end{align}
\end{problem}

\begin{problem}{33}
$y = 2x^2 - 6x + 5, \quad y = x^2 + 6x - 15$
\begin{align}
\descmeet
2x^2 - 6x + 5 &= x^2 + 6x - 15 \\
x^2 - 12x + 20 &= 0 \\
(x - 10)(x - 2) &= 0 \\
x &= 2, 10 \\
\deschigh
2(3)^2 - 6(3) + 5 &= 5 \\
(3)^2 + 6(3) - 15 &= 12 \\
\descarea
A &= \defint{2}{10}{x^2 + 6x - 15} - \defint{2}{10}{2x^2 - 6x + 5} \\
&= \inteval{2}{10}{\frac{x^3}{3} + 3x^2 - 15x} - \inteval{2}{10}{\frac{2x^3}{3} - 3x^2 + 5x} \\
&= \plugin{\frac{(10)^3}{3} + 3(10)^2 - 15(10)}{\frac{(2)^3}{3} + 3(2)^2 - 15(2)} \notag \\
&\quad - \plugin{\frac{2(10)^3}{3} - 3(10)^2 + 5(10)}{\frac{2(2)^3}{3} - 3(2)^2 + 5(2)} \\
&= 85 \frac{1}{3}
\end{align}
\end{problem}

\begin{problem}{35}
$y = 4 - x^2; \quad [-2, 2]$
\begin{align}
y_\text{avg} &= \frac{1}{2 + 2} \defint{-2}{2}{4 - x^2} \\
&= \frac{1}{4} \cdot \inteval{-2}{2}{4x - \frac{x^3}{3}} \\
&= \frac{1}{4} \cdot \plugin{4(2) - \frac{(2)^3}{3}}{4(-2) - \frac{(-2)^3}{3}} \\
&= 2 \frac{2}{3}
\end{align}
\end{problem}

\begin{problem}{53}
$W(t) = -6t^2 + 12t + 90, \quad t \text{ in } [0, 5]$
\begin{align}
\shortintertext{a) Find the speed at the beginning of the interval.}
-(0)t^2 + 12(0) + 90 &= 90 \text{ words per minute} \\
\shortintertext{b) Find the maximum speed and when it occurs.}
W'(t) &= -12t + 12 \\
-12t + 12 &= 0 \\
-12(t - 1) &= 0 \\
t &= 1 \text{ minute} \\
W(1) &= 94 \text{ words per minute, at } t = 1 \text{ minute}
\shortintertext{c) Find the average speed over the 5-min interval}
W_\text{avg} &= \frac{1}{5 - 0} \defint{0}{5}{-6t^2 + 12t + 90} \\
&= \frac{1}{5} \cdot \inteval{0}{5}{-2t^3 + 6t^2 + 90t} \\
&= \frac{1}{5} \cdot \plugin{-2(5)^3 + 6(5)^2 + 90(5)}{-2(0)^3 + 6(0)^2 + 90(0)} \\
&= 70 \text{ words per minute}
\end{align}
\end{problem}

\begin{problem}{60}
$y = e^x, \quad y = e^{-x}, \quad x = -2$
\begin{align}
\descmeet
e^x &= e^{-x} \\
e^x - e^{-x} &= 0 \\
x &= 0
\deschigh
e^{(-1)} &= \frac{1}{e} \\
e^{-(-1)} &= e \\
\descarea
A &= \defint{-2}{0}{e^{-x}} - \defint{-2}{0}{e^{x}} \\
&= \inteval{-2}{0}{-e^{-x}} - \inteval{-2}{0}{e^{x}} \\
&= \plugin{-e^{-(0)}}{-e^{-(-2)}} - \plugin{e^{(0)}}{e^{(-2)}} \\
&\approx 5.524
\end{align}
\end{problem}

\end{document}